erasure/theories/SafeErasureFunction.v
@@ -104,56 +104,334 @@ Ltac sq := try (destruct HΣ as [wfΣ]; clear HΣ);
          | H : ∥ _ ∥ |- _ => destruct H
          end; try eapply sq.
 
+Section Normal.
+
+  Context (flags : RedFlags.t).
+
+  (* TODO: blocked fixes are missing! *)
+  
+  Inductive normal (Γ : context) : term -> Prop :=
+  | nf_ne t : neutral Γ t -> normal Γ t
+  | nf_sort s : normal Γ (tSort s)
+  | nf_prod na A B : normal Γ A -> normal (Γ ,, vass na A) B ->
+                     normal Γ (tProd na A B)
+  | nf_lam na A B : normal Γ A -> normal (Γ ,, vass na A) B ->
+                    normal Γ (tLambda na A B)
+  | nf_cstrapp i n u v : All (normal Γ) v -> normal Γ (mkApps (tConstruct i n u) v)
+  | nf_indapp i u v : All (normal Γ) v -> normal Γ (mkApps (tInd i u) v)
+  | nf_fix mfix idx : All (compose (normal (Γ ,,, fix_context mfix)) dbody) mfix ->
+                      All (compose (normal Γ) dtype) mfix ->
+                      normal Γ (tFix mfix idx)
+  | nf_cofix mfix idx : All (compose (normal (Γ ,,, fix_context mfix)) dbody) mfix ->
+                      All (compose (normal Γ) dtype) mfix ->
+                        normal Γ (tCoFix mfix idx)
+
+  with neutral (Γ : context) : term -> Prop :=
+  | ne_rel i :
+      option_map decl_body (nth_error Γ i) = Some None ->
+      neutral Γ (tRel i)
+  | ne_var v : neutral Γ (tVar v)
+  | ne_evar n l : All (normal Γ) l -> neutral Γ (tEvar n l)
+  | ne_const c u decl :
+      lookup_env Σ c = Some (ConstantDecl c decl) -> decl.(cst_body) = None ->
+      neutral Γ (tConst c u)
+  | ne_app f v : neutral Γ f -> normal Γ v -> neutral Γ (tApp f v)
+  | ne_case i p c brs : neutral Γ c -> normal Γ p -> All (compose (normal Γ) snd) brs ->
+                        neutral Γ (tCase i p c brs)
+  | ne_proj p c : neutral Γ c -> neutral Γ (tProj p c).
+
+End Normal.
+
 Hint Constructors normal neutral.
 
 Derive Signature for normal.
 Derive Signature for neutral.
 
-(* Definition normal_neutral_dec Γ t : ({normal Σ Γ t} + {~ (normal Σ Γ t)}) * ({neutral Σ Γ t} + {~ (neutral Σ Γ t)}). *)
+Ltac d := match goal with
+         | [ H : normal _ (?f ?a) |- _ ] => depelim H
+         | [ H : neutral _ (?f ?a)|- _ ] => depelim H
+         end.
+
+Lemma OnOn2_contra A  (P : A -> A -> Type) l1 l2 : (forall x y, P x y -> False) -> OnOne2 P l1 l2 -> False.
+Proof.
+  intros. induction X; eauto.
+Qed.
+
+Notation decision P := ({P} + {~P}).
+
+Lemma dec_All X (L : list X) P : All (fun x => decision (P x)) L ->
+                                 All P L + (All P L -> False).
+Proof.
+  intros. induction X0.
+  - left. econstructor.
+  - destruct p.
+    + destruct IHX0. firstorder. right. inversion 1. subst. eauto.
+    + right. inversion 1; subst; eauto.
+Defined.
+
+Lemma normal_nf Γ t t' : normal Γ t \/ neutral Γ t -> red1 Σ Γ t t' -> False.
+Proof.
+  intros. induction X using red1_ind_all; destruct H.
+  all: repeat match goal with
+         | [ H : normal _ (?f ?a) |- _ ] => depelim H
+         | [ H : neutral _ (?f ?a)|- _ ] => depelim H
+         end.
+  all: try congruence.
+  Ltac help := try repeat match goal with
+                  | [ H0 : _ = mkApps _ _ |- _ ] => 
+                    eapply (f_equal decompose_app) in H0;
+                      rewrite !decompose_app_mkApps in H0; cbn in *; congruence
+                  | [ H1 : tApp _ _ = mkApps _ ?args |- _ ] =>
+                    destruct args using rev_ind; cbn in *; [ inv H1 |
+                                                             rewrite <- mkApps_nested in H1; cbn in *; inv H1
+                                                    ]
+                  | [ H0 : mkApps _ _ = _ |- _ ] => symmetry in H0
+                         end.
+  all: help.
+  all: try tauto.
+  all: try now (clear - H; depind H; help; eauto).
+  - destruct args using rev_ind; cbn in *; [ inv H1 |
+                                             rewrite <- mkApps_nested in H1; cbn in *; inv H1
+                                           ].
+    destruct narg; inv H3.
+  - eapply OnOne2_All_mix_left in X; try eassumption.
+    eapply OnOn2_contra; try eassumption.
+    firstorder.
+  - eapply OnOne2_All_mix_left in X; try eassumption.
+    eapply OnOn2_contra; try eassumption.
+    firstorder.
+  - eapply IHX. left.
+    eapply nf_cstrapp. now eapply All_app in H as [H _].
+  - eapply IHX. left.
+    eapply nf_indapp. now eapply All_app in H as [H _].
+  - eapply IHX. left.
+    eapply All_app in H as [_ H]. now inv H.
+  - eapply IHX. left.
+    eapply All_app in H as [_ H]. now inv H.
+  - eapply OnOne2_All_mix_left in X; try eassumption.
+    eapply OnOn2_contra; try eassumption.
+    firstorder.
+  - eapply OnOne2_All_mix_left in X; try eassumption.
+    eapply OnOn2_contra; try eassumption.
+    firstorder.
+  - eapply OnOne2_All_mix_left in X; try eassumption.
+    eapply OnOn2_contra; try eassumption.
+    firstorder.
+  - eapply OnOne2_All_mix_left in X. 2:exact H.
+    eapply OnOn2_contra; try eassumption.
+    firstorder.
+  - eapply OnOne2_All_mix_left in X. 2:exact H0.
+    eapply OnOn2_contra; try eassumption.
+    firstorder.
+  - eapply OnOne2_All_mix_left in X. 2:exact H.
+    eapply OnOn2_contra; try eassumption.
+    firstorder.
+Qed.
+
+Hint Constructors normal neutral.
+
+
+Require Import Lia.
+From MetaCoq Require Import PCUIC.PCUICSize.
+
+(* Definition mkApps_decompose_app_rec t l : *)
+(*   mkApps t l = mkApps  (fst (decompose_app_rec t l)) (snd (decompose_app_rec t l)). *)
 (* Proof. *)
-(*   induction t in Γ |- *; split; eauto. *)
-(*   all: try now (right; intros H; depelim H). *)
-(*   - destruct (option_map decl_body (nth_error Γ n)) as [ [ | ] | ] eqn:E. *)
-(*     + right. intros H. depelim H. depelim H. congruence. admit. admit. *)
-(*     + eauto. *)
-(*     + right. intros H. depelim H. depelim H. congruence. admit. admit. *)
-(*   - destruct (option_map decl_body (nth_error Γ n)) as [ [ | ] | ] eqn:E. *)
-(*     + right. intros H. depelim H. congruence.  *)
-(*     + eauto. *)
-(*     + right. intros H. depelim H. congruence. *)
-(*   - destruct (IHt1 Γ) as [[] _]; *)
-(*       [destruct (IHt2 (Γ,, vass na t1)) as [[] _]|]; eauto. *)
-(*     + right. intros H. depelim H. depelim H. eauto. admit. admit. *)
-(*     + right. intros H. depelim H. depelim H. eauto. admit. admit. *)
-(*   - destruct (IHt1 Γ) as [[] _]; *)
-(*       [destruct (IHt2 (Γ,, vass na t1)) as [[] _]|]; eauto. *)
-(*     + right. intros H. depelim H. depelim H. eauto. admit. admit. *)
-(*     + right. intros H. depelim H. depelim H. eauto. admit. admit. *)
-(*   - right. intros H. depelim H. depelim H. admit. admit. *)
-(*   - destruct (IHt1 Γ) as [_ []]; *)
-(*       [destruct (IHt2 Γ) as [[] _]|]; eauto. *)
-(*     + right. intros H. depelim H. depelim H. eauto. admit. admit. *)
-(*     + right. intros H. depelim H. depelim H. eauto. admit. admit. *)
-(*   - destruct (IHt1 Γ) as [_ []]; *)
-(*       [destruct (IHt2 Γ) as [[] _]|]; eauto. *)
-(*     + right. intros H. depelim H. eauto.  *)
-(*     + right. intros H. depelim H. eauto. *)
-(*   - destruct (lookup_env Σ k) as [[] | ] eqn:E. *)
-(*     + destruct (cst_body c) eqn:E2. *)
-(*       * right. intros H. depelim H. depelim H. congruence. admit. admit. *)
-(*       * destruct (string_dec k k0). subst. left. eauto.  *)
-(*         right. intros H. depelim H. depelim H. congruence. admit. admit. *)
-(*     +   right. intros H. depelim H. depelim H. congruence. admit. admit. *)
-(*     +   right. intros H. depelim H. depelim H. congruence. admit. admit. *)
-(*   - destruct (lookup_env Σ k) as [[] | ] eqn:E. *)
-(*     + destruct (cst_body c) eqn:E2. *)
-(*       * right. intros H. depelim H. congruence.  *)
-(*       * destruct (string_dec k k0). subst. left. eauto.  *)
-(*         right. intros H. depelim H. congruence. *)
-(*     +   right. intros H. depelim H. congruence. *)
-(*     +   right. intros H. depelim H. congruence. *)
-(*   - *)
-(* Admitted. *)
+(*   revert l; induction t; try reflexivity. *)
+(*   intro l; cbn in *. *)
+(*   transitivity (mkApps t1 ((t2 ::l))). reflexivity. *)
+(*   now rewrite IHt1. *)
+(* Qed. *)
+
+(* Definition mkApps_decompose_app t : *)
+(*   t = mkApps  (fst (decompose_app t)) (snd (decompose_app t)) *)
+(*   := mkApps_decompose_app_rec t []. *)
+
+Lemma decompose_app_size_tApp1 t1 t2 :
+  size (decompose_app (tApp t1 t2)).1 < size (tApp t1 t2).
+Proof.
+  todo "tApp1".
+Qed.
+
+Lemma decompose_app_size_tApp2 t1 t2 :
+  All (fun t => size t < size (tApp t1 t2)) (decompose_app (tApp t1 t2)).2.
+Proof.
+  todo "tApp2".
+Qed.
+
+Lemma term_forall_mkApps_ind :
+  forall P : term -> Type,
+    (forall n : nat, P (tRel n)) ->
+    (forall i : ident, P (tVar i)) ->
+    (forall (n : nat) (l : list term), All P l -> P (tEvar n l)) ->
+    (forall s, P (tSort s)) ->
+    (forall (n : name) (t : term), P t -> forall t0 : term, P t0 -> P (tProd n t t0)) ->
+    (forall (n : name) (t : term), P t -> forall t0 : term, P t0 -> P (tLambda n t t0)) ->
+    (forall (n : name) (t : term),
+        P t -> forall t0 : term, P t0 -> forall t1 : term, P t1 -> P (tLetIn n t t0 t1)) ->
+    (forall t : term, forall v, ~ isApp t -> P t -> All P v -> P (mkApps t v)) ->
+    (forall (s : String.string) (u : list Level.t), P (tConst s u)) ->
+    (forall (i : inductive) (u : list Level.t), P (tInd i u)) ->
+    (forall (i : inductive) (n : nat) (u : list Level.t), P (tConstruct i n u)) ->
+    (forall (p : inductive * nat) (t : term),
+        P t -> forall t0 : term, P t0 -> forall l : list (nat * term),
+            tCaseBrsProp P l -> P (tCase p t t0 l)) ->
+    (forall (s : projection) (t : term), P t -> P (tProj s t)) ->
+    (forall (m : mfixpoint term) (n : nat), tFixProp P P m -> P (tFix m n)) ->
+    (forall (m : mfixpoint term) (n : nat), tFixProp P P m -> P (tCoFix m n)) ->
+    forall t : term, P t.
+Proof.
+  intros until t.
+  assert (Acc (MR lt size) t) by eapply measure_wf, Wf_nat.lt_wf.
+  induction H. rename X14 into auxt. clear H. rename x into t.
+  move auxt at top.
+
+  destruct t; try now repeat (match goal with
+                 H : _ |- _ => apply H; try (hnf; cbn; lia)
+              end).
+
+  - eapply X1. revert l auxt. unfold MR; cbn. fix auxt' 1.
+    destruct l; constructor. apply auxt. hnf; cbn; lia. apply auxt'. intros. apply auxt.
+    hnf in *; cbn in *. lia. 
+
+  - rewrite mkApps_decompose_app.
+    destruct decompose_app eqn:E. cbn.
+    eapply X6.
+    + eapply decompose_app_notApp in E. eauto.
+    + eapply auxt. cbn. hnf. pose proof (decompose_app_size_tApp1 t1 t2). rewrite E in *. hnf in *; cbn in *. lia.
+    + pose proof (decompose_app_size_tApp2 t1 t2). rewrite E in *. cbn in H. clear E.
+      induction l.
+      * econstructor.
+      * inv H. econstructor. eapply auxt. hnf; cbn. eassumption.
+        eapply IHl. eassumption.
+        
+  - eapply X10; [apply auxt; hnf; cbn; lia.. | ]. rename brs into l.
+    revert l auxt. unfold MR; cbn. fix auxt' 1.
+    destruct l; constructor. apply auxt. hnf; cbn; lia. apply auxt'. intros. apply auxt.
+    hnf in *; cbn in *. lia. 
+  
+  - eapply X12; [apply auxt; hnf; cbn; lia.. | ]. rename mfix into l.
+    revert l auxt. unfold MR; cbn. fix auxt' 1.
+    destruct l; constructor. split.
+    apply auxt. hnf; cbn. unfold def_size. lia.
+    apply auxt. hnf; cbn. unfold def_size. lia.   
+    apply auxt'. intros. apply auxt.
+    hnf in *; cbn in *. unfold mfixpoint_size, def_size in *. lia. 
+
+  - eapply X13; [apply auxt; hnf; cbn; lia.. | ]. rename mfix into l.
+    revert l auxt. unfold MR; cbn. fix auxt' 1.
+    destruct l; constructor. split.
+    apply auxt. hnf; cbn. unfold def_size. lia.
+    apply auxt. hnf; cbn. unfold def_size. lia.   
+    apply auxt'. intros. apply auxt.
+    hnf in *; cbn in *. unfold mfixpoint_size, def_size in *. lia. 
+Defined.
+
+Definition normal_neutral_dec Γ t : ({normal Γ t} + {~ (normal Γ t)}) * ({neutral Γ t} + {~ (neutral Γ t)}).
+Proof.
+  induction t using term_forall_mkApps_ind in Γ |- *; split; eauto.
+  all: try now (right; intros H; depelim H).
+  - destruct (option_map decl_body (nth_error Γ n)) as [ [ | ] | ] eqn:E.
+    + right. intros H. depelim H. depelim H. congruence. help. help.
+    + eauto.
+    + right. intros H. depelim H. depelim H. congruence. help. help.
+  - destruct (option_map decl_body (nth_error Γ n)) as [ [ | ] | ] eqn:E.
+    + right. intros H. depelim H. congruence.
+    + eauto.
+    + right. intros H. depelim H. congruence.
+  - todo "evar".
+  - todo "evar".
+  - destruct (IHt1 Γ) as [[] _];
+      [destruct (IHt2 (Γ,, vass n t1)) as [[] _]|]; eauto.
+    + right. intros H. depelim H. depelim H. eauto. help. help.
+    + right. intros H. depelim H. depelim H. eauto. help. help.
+  - destruct (IHt1 Γ) as [[] _];
+      [destruct (IHt2 (Γ,, vass n t1)) as [[] _]|]; eauto.
+    + right. intros H. depelim H. depelim H. eauto. help. help.
+    + right. intros H. depelim H. depelim H. eauto. help. help.
+  - right. intros H. depelim H. depelim H. help. help.
+  - destruct t.
+    11:{
+      destruct dec_All with (P := (normal Γ)) (L := v).
+      - eapply All_impl. eassumption. intros ? ?. apply H1.
+      - left. eauto.
+      - right. clear - f. intros ?. depelim H.
+        depelim H. all:try now help. todo "TODO".
+    }
+
+    10:{
+      destruct dec_All with (P := (normal Γ)) (L := v).
+      - eapply All_impl. eassumption. intros ? ?. apply H1.
+      - left. eauto.
+      - right. clear - f. intros ?. depelim H.
+        depelim H. all:try now help. help. todo "TODO".
+      
+    }
+
+    all:right; todo "TODO".
+    
+    (* right. intros Hn. depelim Hn. depelim H1. all:help. admit. admit. *)
+    (* right. intros Hn. depelim Hn. depelim H1. all:help. admit. admit. *)
+  - destruct v using rev_ind.
+    + cbn. eapply IHt.
+    + rewrite <- mkApps_nested. cbn.
+      eapply All_app in H0 as []. eapply IHv in a. inv a0. clear H3.
+      rename H2 into IHt2.
+      revert a.
+      generalize (mkApps t v) as t1. intros t1 IHt1.
+      destruct (IHt1) as [];
+      [destruct (IHt2 Γ) as [[] _]|]; eauto.
+      * right. intros HH. depelim HH. eauto.
+      * right. intros HH. depelim HH. eauto.
+  - destruct (lookup_env Σ s) as [[] | ] eqn:E.
+    + destruct (cst_body c) eqn:E2.
+      * right. intros H. depelim H. depelim H. congruence. help. help.
+      * destruct (string_dec s k). subst. left. eauto.
+        right. intros H. depelim H. depelim H. congruence. help. help.
+    +   right. intros H. depelim H. depelim H. congruence. help. help.
+    +   right. intros H. depelim H. depelim H. congruence. help. help.
+  - destruct (lookup_env Σ s) as [[] | ] eqn:E.
+    + destruct (cst_body c) eqn:E2.
+      * right. intros H. depelim H. congruence.
+      * destruct (string_dec s k). subst. left. eauto.
+        right. intros H. depelim H. congruence.
+    +   right. intros H. depelim H. congruence.
+    +   right. intros H. depelim H. congruence.
+  - left. eapply nf_indapp with (v := []). econstructor.
+  - left. eapply nf_cstrapp with (v := []). econstructor.
+  - todo "case".
+  - todo "case".
+  - destruct (IHt Γ) as [_ []].
+    + eauto.
+    + right. intros H. depelim H. depelim H. eauto. help. help.
+  - destruct (IHt Γ) as [_ []].
+    + eauto.
+    + right. intros H. depelim H. eauto.
+  - hnf in X.
+
+    destruct dec_All with (P := (normal Γ ∘ dtype)) (L := m).
+    eapply All_impl. eassumption. cbn. intros. eapply H.
+
+    destruct dec_All with (P := normal (Γ ,,, fix_context m) ∘ dbody) (L := m).
+    eapply All_impl. exact X. cbn. intros. eapply H.
+
+    + left. eapply nf_fix. eauto. eauto.
+    + right. intros H. depelim H. depelim H. help. help. eauto.
+    + right. intros H. depelim H. depelim H. help. help. eauto.
+  - hnf in X.
+
+    destruct dec_All with (P := (normal Γ ∘ dtype)) (L := m).
+    eapply All_impl. eassumption. cbn. intros. eapply H.
+
+    destruct dec_All with (P := normal (Γ ,,, fix_context m) ∘ dbody) (L := m).
+    eapply All_impl. exact X. cbn. intros. eapply H.
+
+    + left. eapply nf_cofix. eauto. eauto.
+    + right. intros H. depelim H. depelim H. help. help. eauto.
+    + right. intros H. depelim H. depelim H. help. help. eauto.
+Defined.
+
+Definition normal_dec Γ t := fst (normal_neutral_dec Γ t).
 
 Lemma mkApps_tFix_inv t mfix n L :
   t = mkApps (tFix mfix n) L ->
@@ -168,58 +446,58 @@ Proof.
 Qed.
 
 Notation err := (TypeError  (Msg "hnf did not return normal form")).
-Program Fixpoint normal_dec Γ t : typing_result (forall t', red1 Σ Γ t t' -> False) :=
-  match t with
-  | tRel n => match option_map decl_body (nth_error Γ n) with
-               Some (Some body) => err
-             | _ => ret _
-             end
-  | tVar n => ret _
-  | tSort u => ret _
-  | tProd na A B => H1 <- normal_dec Γ A ;;
-                      H2 <- normal_dec (Γ,, vass na A) B;;
-                      ret _
-  | tLambda na A B => H1 <- normal_dec Γ A ;;
-                      H2 <- normal_dec (Γ,, vass na A) B;;
-                      ret _
-  | tLetIn _ _ _ _ => err
-  | tConst c u => match lookup_env Σ c  with Some (ConstantDecl _ (Build_constant_body _ (Some _) _)) => err
-                                       | _ => ret _
-                 end
-  | tInd _ _ => ret _
-  | tConstruct _ _ _ => ret _
-  | tCase _ _ _ _ => err
-  | tProj _ _ => err
-  (* | tFix _ _ => ret _ *)
-  (* | tCoFix _ _ => ret _ *)
-  | _ => TypeError (Msg "not implemented")
-  end.
-Next Obligation.
-  intros; depelim X; try congruence; eapply mkApps_tFix_inv in H0 as [(? & ? & ?) | [] ]; congruence.
-Qed.
-Next Obligation.
-  intros; depelim X; try congruence; try eapply mkApps_tFix_inv in H as [(? & ? & ?) | [] ]; try congruence.
-Qed.
-Next Obligation.
-  intros; depelim X; try congruence; try eapply mkApps_tFix_inv in H as [(? & ? & ?) | [] ]; try congruence.
-Qed.
-Next Obligation.
-  intros; depelim X; try congruence; try eapply mkApps_tFix_inv in H as [(? & ? & ?) | [] ]; try congruence; eauto.
-Qed.
-Next Obligation.
-  intros; depelim X; try congruence; try eapply mkApps_tFix_inv in H as [(? & ? & ?) | []]; try congruence; eauto.
-Qed.
-Next Obligation.
-  intros; depelim X; try congruence; try eapply mkApps_tFix_inv in H0 as [(? & ? & ?) | [] ]; try congruence; eauto.
-  unfold declared_constant in *. rewrite isdecl in H. destruct decl. destruct cst_body; cbn in *; firstorder congruence.
-Qed.
-Next Obligation.
-  intros; depelim X; try congruence; try eapply mkApps_tFix_inv in H as [(? & ? & ?) | [] ]; try congruence; eauto.
-Qed.
-Next Obligation.
-  intros; depelim X; try congruence; try eapply mkApps_tFix_inv in H as [(? & ? & ?) | [] ]; try congruence; eauto.
-Qed.
-Solve All Obligations with firstorder congruence.
+(* Program Fixpoint normal_dec Γ t : typing_result (forall t', red1 Σ Γ t t' -> False) := *)
+(*   match t with *)
+(*   | tRel n => match option_map decl_body (nth_error Γ n) with *)
+(*                Some (Some body) => err *)
+(*              | _ => ret _ *)
+(*              end *)
+(*   | tVar n => ret _ *)
+(*   | tSort u => ret _ *)
+(*   | tProd na A B => H1 <- normal_dec Γ A ;; *)
+(*                       H2 <- normal_dec (Γ,, vass na A) B;; *)
+(*                       ret _ *)
+(*   | tLambda na A B => H1 <- normal_dec Γ A ;; *)
+(*                       H2 <- normal_dec (Γ,, vass na A) B;; *)
+(*                       ret _ *)
+(*   | tLetIn _ _ _ _ => err *)
+(*   | tConst c u => match lookup_env Σ c  with Some (ConstantDecl _ (Build_constant_body _ (Some _) _)) => err *)
+(*                                        | _ => ret _ *)
+(*                  end *)
+(*   | tInd _ _ => ret _ *)
+(*   | tConstruct _ _ _ => ret _ *)
+(*   | tCase _ _ _ _ => err *)
+(*   | tProj _ _ => err *)
+(*   (* | tFix _ _ => ret _ *) *)
+(*   (* | tCoFix _ _ => ret _ *) *)
+(*   | _ => TypeError (Msg "not implemented in normality decider") *)
+(*   end. *)
+(* Next Obligation. *)
+(*   intros; depelim X; try congruence; eapply mkApps_tFix_inv in H0 as [(? & ? & ?) | [] ]; congruence. *)
+(* Qed. *)
+(* Next Obligation. *)
+(*   intros; depelim X; try congruence; try eapply mkApps_tFix_inv in H as [(? & ? & ?) | [] ]; try congruence. *)
+(* Qed. *)
+(* Next Obligation. *)
+(*   intros; depelim X; try congruence; try eapply mkApps_tFix_inv in H as [(? & ? & ?) | [] ]; try congruence. *)
+(* Qed. *)
+(* Next Obligation. *)
+(*   intros; depelim X; try congruence; try eapply mkApps_tFix_inv in H as [(? & ? & ?) | [] ]; try congruence; eauto. *)
+(* Qed. *)
+(* Next Obligation. *)
+(*   intros; depelim X; try congruence; try eapply mkApps_tFix_inv in H as [(? & ? & ?) | []]; try congruence; eauto. *)
+(* Qed. *)
+(* Next Obligation. *)
+(*   intros; depelim X; try congruence; try eapply mkApps_tFix_inv in H0 as [(? & ? & ?) | [] ]; try congruence; eauto. *)
+(*   unfold declared_constant in *. rewrite isdecl in H. destruct decl. destruct cst_body; cbn in *; firstorder congruence. *)
+(* Qed. *)
+(* Next Obligation. *)
+(*   intros; depelim X; try congruence; try eapply mkApps_tFix_inv in H as [(? & ? & ?) | [] ]; try congruence; eauto. *)
+(* Qed. *)
+(* Next Obligation. *)
+(*   intros; depelim X; try congruence; try eapply mkApps_tFix_inv in H as [(? & ? & ?) | [] ]; try congruence; eauto. *)
+(* Qed. *)
+(* Solve All Obligations with firstorder congruence. *)
 
 Inductive red' (Σ : global_env) (Γ : context) : term -> term -> Type :=
   refl_red' M : red' Σ Γ M M
@@ -246,7 +524,7 @@ Program Definition reduce_to_sort' Γ t (h : wellformed Σ Γ t)
   | _ =>
     match hnf HΣ Γ t h with
     | tSort u => ret (inl (u; _))
-    | t' => match normal_dec Γ t' with Checked H => ret (inr _) | TypeError t => TypeError t end
+    | t' => match normal_dec Γ t' with left H => ret (inr _) | right t => err end
     end
   end.
 Next Obligation.
@@ -262,7 +540,7 @@ Next Obligation.
   inversion r; subst.
   - eapply invert_red_sort in r0; eauto.
     edestruct H0. eauto.
-  - eauto.
+  - eapply normal_nf. left; eassumption. eauto.    
 Qed.
 
 Program Definition reduce_to_prod' Γ t (h : wellformed Σ Γ t)
@@ -272,7 +550,7 @@ Program Definition reduce_to_prod' Γ t (h : wellformed Σ Γ t)
   | _ =>
     match hnf HΣ Γ t h with
     | tProd na a b => ret (inl (na; a; b; _))
-    | t' => match normal_dec Γ t' with Checked H => ret (inr _) | _ => TypeError (Msg "hnf did not return normal form") end
+    | t' => match normal_dec Γ t' with left H => ret (inr _) | right t => err end
     end
   end.
 Next Obligation.
@@ -288,7 +566,7 @@ Next Obligation.
   inversion r; subst.
   - eapply invert_red_prod in r0 as (? & ? & [] & ?); eauto.
     edestruct H0. eauto.
-  - eauto.
+  - eapply normal_nf. left; eassumption. eauto.    
 Qed.
 
 Equations is_arity Γ (HΓ : ∥wf_local Σ Γ∥) T (HT : wellformed Σ Γ T) :
